make everything compile again (except Pipeline and PipelineTest)

src/Memory.v
@@ -1,19 +1,17 @@
 Require Import bbv.Word.
+Require Import riscv.RiscvBitWidths.
 Require Import compiler.Common.
 
 Section Memory.
 
-  Context {w: nat}.
+  Context {Bw: RiscvBitWidths}.
 
-  Definition mem := word w -> option (word w).
+  Definition mem := word wXLEN -> option (word wXLEN).
 
-  Definition alignment: nat :=
-    if dec (w = 64) then 8 else if dec (w = 32) then 4 else 0.
-  
-  Definition read_mem(x: word w)(m: mem): option (word w) :=
-    if dec ((wordToNat x) mod alignment = 0) then m x else None.
+  Definition read_mem(x: word wXLEN)(m: mem): option (word wXLEN) :=
+    if dec ((wordToNat x) mod wXLEN_in_bytes = 0) then m x else None.
 
-  Definition write_mem(x: word w)(v: word w)(m: mem): option (mem) :=
+  Definition write_mem(x: word wXLEN)(v: word wXLEN)(m: mem): option (mem) :=
     match read_mem x m with
     | Some old_value => Some (fun y => if dec (x = y) then Some v else m y)
     | None => None
@@ -21,6 +19,6 @@ Section Memory.
 
   Definition no_mem: mem := fun x => None.
 
-  Definition zeros_mem(upTo: word w): mem := fun x => if wlt_dec x upTo then Some $0 else None.
+  Definition zeros_mem(upTo: word wXLEN): mem := fun x => if wlt_dec x upTo then Some $0 else None.
 
 End Memory.
